\documentclass{article}
\usepackage{eecstex}
\usepackage{pgfplots}

\title{EE 120 HW 03}
\author{Bryan Ngo}
\date{2021-02-10}

\begin{document}

\maketitle

\section{LTI Statements}

\begin{enumerate}
    \item False, consider the system \(y[n] = nx[n]\). This is causal, but is not bounded by some \(B_x\).
    \item False, consider the system \(h[n] = \frac{1}{n}\) over the domain \([-2, 2]\), which is finite but diverges to infinity at \(n = 0\).
    \item True, this means that \(h(t)\) is not absolutely integrable, since the absolute value means that we are integrating strictly positive values over all of \(\R\).
    \item False, consider \(h[n] = 1 \leqslant 2\), then \(\sum_{k \in \Z} h[k]\) diverges.
    \item True, the convolution of the impulse and step response can cut the domain to strictly the nonnegative integers, which implies that \(s[n] = 0\) for all \(n < 0\).
\end{enumerate}

\section{Impulse Response of Discrete Time LTI Systems}

\subsection{}

\begin{equation}
    h[n] = \alpha^n u[n]
\end{equation}
\textbf{Stability}:
\begin{equation}
    \sum_{k \in \Z} \alpha^k u[k] = \sum_{k \geqslant 0} \alpha^k = \frac{1}{1 - \alpha}
\end{equation}
\textbf{Causality}: The system is causal since \(h[n] = 0\) for \(n < 0\).

\subsection{}

\begin{equation}
    h[n] = \beta^n u[3 - n]
\end{equation}
\textbf{Stability}:
\begin{equation}
    \sum_{k \in \Z} \beta^k u[3 - k] = \sum_{k \leqslant 3} \beta^k = \sum_{k \in [0, 2]} \beta^k + \sum_{k \geqslant 0} \left(\frac{1}{\beta}\right)^k = 1 + \beta + \beta^2 + \frac{1}{1 - \frac{1}{\beta}}
\end{equation}
\textbf{Causality}: The system is \emph{not} causal since \(h[n] \neq 0\) for \(n = -1\), for example.

\subsection{}

\begin{equation}
    h[n] = n (0.6)^n u[n]
\end{equation}
\textbf{Stability}:
\begin{equation}
    \sum_{k \in \Z} k (0.6)^k u[k] = \sum_{k \geqslant 0} k (0.6)^k
\end{equation}
Observe that the series converges. \\ % TODO: how?
\textbf{Causality}: The system is causal since \(h[n] = 0\) for \(n < 0\), for example.

\subsection{}

\begin{equation}
    h[n] = u[n] - u[n + 100]
\end{equation}
\textbf{Stability}: Note that this is a flipped rectangle function shifted to the domain \([-100, 0]\), meaning that its \(\sum_{k \in \Z} |h[k]| = 100\). \\
\textbf{Causality}: The system is \emph{not} causal since \(h[n] = -1\) for \(n \in [-100, 0]\).

\section{Impulse Response of Continuous Time LTI systems}

\subsection{}

\begin{equation}
    h(t) = e^{-3t} u(t - 5)
\end{equation}
\textbf{Stability}: The integral is
\begin{equation}
    \int_{\R} |h(t)| \, dt = \int_5^\infty e^{-3t} \, dt = \left.-\frac{1}{3} e^{-3t}\right|_5^\infty = \frac{e^{-15}}{3}
\end{equation}
\textbf{Causality}: The system is causal since \(h(t) = 0\) for \(t < 5\).

\subsection{}

\begin{equation}
    h(t) = e^{-4t} u(3 - t)
\end{equation}
\textbf{Stability}: The integral is
\begin{equation}
    \int_{\R} |h(t)| \, dt = \int_{-\infty}^3 e^{-4t} \, dt = \left.-\frac{1}{4} e^{-4t}\right|_{-\infty}^3
\end{equation}
which diverges. \\
\textbf{Causality}: The system is \emph{not} causal since \(h(t) = e^4\) for \(t = -1\).

\subsection{}

\begin{equation}
    h(t) = e^{-4|t|}
\end{equation}
\textbf{Stability}: The integral is
\begin{align}
    \int_{\R} e^{-4|t|} \, dt &= \int_{-\infty}^0 e^{4t} \, dt + \int_0^\infty e^{-4t} \, dt \\
    &= 2 \int_0^\infty e^{-4t} \, dt = \left.-\frac{1}{2} e^{-4t}\right|_0^\infty = \frac{1}{2}
\end{align}
\textbf{Causality}: The system is \emph{not} causal since \(h(t) = e^{-4}\) for \(t = -1\).

\subsection{}

\begin{equation}
    h(t) = t e^{-t} u(t)
\end{equation}
\textbf{Stability}: The integral is
\begin{align}
    \int_{\R} |h(t)| \, dt = \int_0^\infty t e^{-t} \, dt = \left.-(t + 1) e^{-t}\right|_0^\infty = 1
\end{align}
\textbf{Causality}: The system is causal since \(h(t) = 0\) for \(t < 0\).

\section{LTI System Impulse Response}

\begin{align}
    h_1[n] &= \sin[8n] \\
    h_2[n] &= a^n u[n] \\
    x[n] &= \delta[n] - a \delta[n - 1]
\end{align}
By the properties of convolution,
\begin{equation}
    y[n] = (h_2[n] \ast h_1[n]) \ast x[n]
\end{equation}
Finding what \((h_2 \ast x)[n]\) is,
\begin{align}
    a^n u[n] \ast (\delta[n] - a\delta[n - 1]) = a^n u[n] - a^{n - 1} a u[n - 1] = a^n (u[n] - u[n - 1]) = a^n \delta[n] = \delta[n]
\end{align}
where we can eliminate the exponential term because the function is only nonzero at \(n = 0\), so \(a^0 = 1\).
Then, finding the final convolution,
\begin{equation}
    \delta[n] \ast \sin[8n] = \sin[8n]
\end{equation}

\section{Manual Convolution}

\subsection{}

\begin{equation}
    (x + w) \ast y = (x \ast y) + (w \ast y)
\end{equation}
Plotting \((x + w) \ast y\),
\begin{center}
    \begin{tikzpicture}
        \begin{axis}[
            xlabel=\(n\), ylabel={\(x + w\)},
            axis lines=middle,
            ymin=-3, ymax=3,
            width=0.4\textwidth
        ]
        \addplot[
            ycomb,
            color=blue,
            mark=*
        ]
        coordinates {
            (-3, 0)
            (-2, 0)
            (-1, 0)
            (0, 2)
            (1, 3)
            (2, 0)
            (3, 0)
        };
        \end{axis}
    \end{tikzpicture}
    \begin{tikzpicture}
        \begin{axis}[
            xlabel=\(n\), ylabel={\((x + w) \ast y\)},
            axis lines=middle,
            ymin=-3, ymax=3,
            width=0.4\textwidth
        ]
        \addplot[
            ycomb,
            color=blue,
            mark=*
        ]
        coordinates {
            (-3, 0)
            (-2, 0)
            (-1, 2)
            (0, 3)
            (1, -2)
            (2, -3)
            (3, 0)
        };
        \end{axis}
    \end{tikzpicture}
\end{center}
Likewise, plotting \(x \ast y\) and \(w \ast y\),
\begin{center}
    \begin{tikzpicture}
        \begin{axis}[
            xlabel=\(n\), ylabel={\(x \ast y\)},
            axis lines=middle,
            ymin=-3, ymax=3,
            width=0.4\textwidth
        ]
        \addplot[
            ycomb,
            color=blue,
            mark=*
        ]
        coordinates {
            (-3, 0)
            (-2, 0)
            (-1, 1)
            (0, 2)
            (1, -1)
            (2, -2)
            (3, 0)
        };
        \end{axis}
    \end{tikzpicture}
    \begin{tikzpicture}
        \begin{axis}[
            xlabel=\(n\), ylabel={\(w \ast y\)},
            axis lines=middle,
            ymin=-3, ymax=3,
            width=0.4\textwidth
        ]
        \addplot[
            ycomb,
            color=blue,
            mark=*
        ]
        coordinates {
            (-3, 0)
            (-2, 0)
            (-1, 1)
            (0, 1)
            (1, -1)
            (2, -1)
            (3, 0)
        };
        \end{axis}
    \end{tikzpicture}
\end{center}
As observed, their sum is equal to the above plot, so the distributive property holds.

\subsection{}

\begin{equation}
    (x \ast y) \cdot w \neq x \ast (y \cdot w)
\end{equation}
Drawing these two plots,
\begin{center}
    \begin{tikzpicture}
        \begin{axis}[
            xlabel=\(n\), ylabel={\((x \ast y) \cdot w\)},
            axis lines=middle,
            ymin=-3, ymax=3,
            width=0.4\textwidth
        ]
        \addplot[
            ycomb,
            color=blue,
            mark=*
        ]
        coordinates {
            (-3, 0)
            (-2, 0)
            (-1, 0)
            (0, 2)
            (1, -1)
            (2, 0)
            (3, 0)
        };
        \end{axis}
    \end{tikzpicture}
    \begin{tikzpicture}
        \begin{axis}[
            xlabel=\(n\), ylabel={\(x \ast (y \cdot w)\)},
            axis lines=middle,
            ymin=-3, ymax=3,
            width=0.4\textwidth
        ]
        \addplot[
            ycomb,
            color=blue,
            mark=*
        ]
        coordinates {
            (-3, 0)
            (-2, 0)
            (-1, 0)
            (0, 0)
            (1, -1)
            (2, -2)
            (3, 0)
        };
        \end{axis}
    \end{tikzpicture}
\end{center}
which are clearly not equal.

\section{Convolution \& Correlation}

\begin{align}
    x(t) &=
    \begin{cases}
        2 & t \in (0, 3) \\
        0 & \text{elsewhere}
    \end{cases} \\
    g(t) &= e^{-\frac{t}{2}} u(t)
\end{align}

\subsection{}

\begin{align}
    x(t) \ast g(t) &= \int_{\R} x(\tau) e^{-\frac{1}{2} (t - \tau)} u(t - \tau) \, d\tau \\
    &= \int_0^3 2e^{-\frac{1}{2} (t - \tau)} u(t - \tau) \, d\tau \\
    &= \int_0^t 2e^{-\frac{1}{2} (t - \tau)} \, d\tau + \cancelto{0}{\int_t^3 2e^{-\frac{1}{2} (t - \tau)} u(t - \tau) \, d\tau} \\
    &= \left.4e^{-\frac{1}{2} (t - \tau)}\right|_0^t = 4(1 - e^{-\frac{1}{2} t})
\end{align}
Plotting the convolution,
\begin{center}
    \begin{tikzpicture}
        \begin{axis}[
            xlabel=\(t\), ylabel={\(4e^{-\frac{1}{2} t} - 4\)},
            axis lines=middle,
            xmin=-2, xmax=4,
            title={\((x \ast g)(t)\)},
            width=0.4\textwidth
        ]
        \addplot[
            color=blue,
        ]{4 - 4*exp(-x/2)};
        \end{axis}
    \end{tikzpicture}
\end{center}

\subsection{}

\begin{align}
    x(t) \circ g(t) &= \int_{\R} x(\tau) e^{-\frac{1}{2} (t + \tau)} u(t + \tau) \, d\tau \\
    &= \int_0^3 2e^{-\frac{1}{2} (t + \tau)} u(t + \tau) \, d\tau \\
    &= \cancelto{0}{\int_0^{-t} 2e^{-\frac{1}{2} (t + \tau)} u(t + \tau) \, d\tau} + \int_{-t}^3 2e^{-\frac{1}{2} (t + \tau)} \, d\tau \\
    &= \left.-4e^{-\frac{1}{2} (t + \tau)}\right|_{-t}^3 = -4(e^{-\frac{1}{2} (t + 3)} - 1)
\end{align}
Plotting the cross-correlation,
\begin{center}
    \begin{tikzpicture}
        \begin{axis}[
            xlabel=\(t\), ylabel={\(-4(e^{-\frac{1}{2} (t + 3)} - 1)\)},
            axis lines=middle,
            title={\((x \circ g)(t)\)},
            width=0.4\textwidth
        ]
        \addplot[
            color=blue,
        ]{4 - 4*exp(-(x + 3) / 2)};
        \end{axis}
    \end{tikzpicture}
\end{center}

\subsection{}

\begin{align}
    g(t) \circ x(t) &= \int_{\R} e^{-\frac{1}{2} \tau} u(\tau) x(t + \tau) \, d\tau \\
    &= \int_0^\infty e^{-\frac{1}{2} \tau} x(t + \tau) \, d\tau \\
    &= \int_{-t}^{3 - t} 2e^{-\frac{1}{2} \tau} \, d\tau \\
    &= \left.-4e^{-\frac{1}{2} \tau}\right|_{-t}^{3 - t} = -4(e^{\frac{1}{2} (t - 3)} - e^{\frac{1}{2} t}) = -4e^{\frac{t}{2} t} (e^{-\frac{3}{2}} - 1)
\end{align}
Plotting the cross-correlation,
\begin{center}
    \begin{tikzpicture}
        \begin{axis}[
            xlabel=\(t\), ylabel={\(-4e^{\frac{t}{2} t} (e^{-\frac{3}{2}} - 1)\)},
            axis lines=middle,
            title={\((x \circ g)(t)\)},
            width=0.4\textwidth
        ]
        \addplot[
            color=blue,
        ]{-4*exp{x/2}*(exp(-3/2) - 1)};
        \end{axis}
    \end{tikzpicture}
\end{center}

\subsection{}

Intuitively, convolution measures the effect one signal has on another.
Meanwhile, cross-correlation measures how similar two signals are to each other.
Mathematically,
\begin{equation}
    x(t) \circ y(t) = x(t) \ast y(-t)
\end{equation}

\section{Convolution Practice}

\subsection{}

\begin{center}
    \begin{tikzpicture}
        \begin{axis}[
            xlabel=\(n\), ylabel={\(x[n] - \alpha x[n - 1]\)},
            title={\(g[n]\), \(\alpha = \frac{1}{2}\)},
            axis lines=middle,
            ymin=0, ymax=1
        ]
        \addplot[ycomb, mark=*, color=blue] table[
            col sep=comma,
            x=n, y=gn
        ]{q7-1.csv};
        \end{axis}
    \end{tikzpicture}
\end{center}
We can rewrite \(g[n]\) as
\begin{equation}
    g[n] = x[n] \ast (\delta[n] - \alpha \delta[n - 1])
\end{equation}

\subsection{}

Let \(h[n] = \delta[n + 2] - \left(\frac{1}{2}\right)^4 \delta[n - 2]\) and let \(x[n] = \left(\frac{1}{2}\right)^{n - 2} u[n]\).

\end{document}
